cedar-lean/Cedar/Thm/Validation/Levels/Set.lean
@@ -32,7 +32,7 @@ theorem level_based_slicing_is_sound_set {xs : List Expr} {n : Nat} {c₀ c₁: 
   (hc : CapabilitiesInvariant c₀ request entities)
   (hr : RequestAndEntitiesMatchEnvironment env request entities)
   (ht : typeOf (.set xs) c₀ env = Except.ok (tx, c₁))
-  (hl : TypedExpr.AtLevel tx n)
+  (hl : TypedExpr.AtLevel tx env n)
   (ih : ∀ x ∈ xs, TypedAtLevelIsSound x) :
   evaluate (.set xs) request entities = evaluate (.set xs) request slice
 := by
