cedar-lean/Cedar/Thm/Validation/Slice/BinaryApp.lean
@@ -60,7 +60,7 @@ theorem checked_eval_entity_reachable_get_tag {e₁ e₂: Expr} {n : Nat} {c c' 
   (hc : CapabilitiesInvariant c request entities)
   (hr : RequestAndEntitiesMatchEnvironment env request entities)
   (ht : typeOf (.binaryApp .getTag e₁ e₂) c env = .ok (tx, c'))
-  (hl : TypedExpr.EntityAccessAtLevel tx n nmax path)
+  (hl : TypedExpr.EntityAccessAtLevel tx env n nmax path)
   (he : evaluate (.binaryApp .getTag e₁ e₂) request entities = .ok v)
   (ha : Value.EuidViaPath v path euid)
   (ih₁ : CheckedEvalEntityReachable e₁) :
@@ -115,7 +115,7 @@ theorem checked_eval_entity_reachable_binary {op : BinaryOp} {e₁ e₂: Expr} {
   (hc : CapabilitiesInvariant c request entities)
   (hr : RequestAndEntitiesMatchEnvironment env request entities)
   (ht : typeOf (.binaryApp op e₁ e₂) c env = .ok (tx, c'))
-  (hl : TypedExpr.EntityAccessAtLevel tx n nmax path)
+  (hl : TypedExpr.EntityAccessAtLevel tx env n nmax path)
   (he : evaluate (.binaryApp op e₁ e₂) request entities = .ok v)
   (ha : Value.EuidViaPath v path euid)
   (ih₁ : CheckedEvalEntityReachable e₁) :
